internalize perm into ArrayPtr

ulib/experimental/Steel.ArrayPtr.fst
@@ -43,13 +43,15 @@ type t (a: Type u#0) = {
   base: A.array1 a;
   from: U32.t;
   to: ghost_ref (to_v base from);
+  rperm: ghost_ref perm;
 }
 
-let mk_t (#a: Type u#0) (base: A.array1 a) (from: U32.t) (to: ghost_ref (to_v base from)) : Tot (t a) =
+let mk_t (#a: Type u#0) (base: A.array1 a) (from: U32.t) (to: ghost_ref (to_v base from)) (perm: ghost_ref perm) : Tot (t a) =
   {
     base = base;
     from = from;
     to = to;
+    rperm = perm;
   }
 
 let array_of
@@ -65,96 +67,152 @@ let array_of
 
 let varrayptr0_dep
   (#a: Type)
-  (q: perm)
   (p: t a)
-  (to: normal (t_of (ghost_vptr p.to)))
+  (to_perm: normal (t_of (ghost_vptr p.to `star` ghost_vptr p.rperm)))
 : Tot vprop
-= A.varrayp (array_of p to) q
+= A.varrayp (array_of p (fst to_perm)) (snd to_perm)
 
 let varrayptr0_rewrite
   (#a: Type)
-  (q: perm)
   (p: t a)
-  (x: normal (t_of (ghost_vptr p.to `vdep` varrayptr0_dep q p)))
+  (x: normal (t_of ((ghost_vptr p.to `star` ghost_vptr p.rperm) `vdep` varrayptr0_dep p)))
 : Tot (v a)
-= let (| to, contents |) = x in
+= let (| to_perm, contents |) = x in
   {
-    array = array_of p to;
+    array = array_of p (fst to_perm);
     contents = contents;
+    perm = snd to_perm;
   }
 
+[@@ __steel_reduce__; __reduce__ ]
 let varrayptr0
   (#a: Type)
   (r: t a)
-  (p: perm)
 : Tot vprop
-= (ghost_vptr r.to `vdep` varrayptr0_dep p r) `vrewrite` varrayptr0_rewrite p r
+= ((ghost_vptr r.to `star` ghost_vptr r.rperm) `vdep` varrayptr0_dep r) `vrewrite` varrayptr0_rewrite r
 
-let is_arrayptr #a r p = hp_of (varrayptr0 r p)
+let is_arrayptr #a r = hp_of (varrayptr0 r)
 
-let arrayptr_sel #a r p = fun h -> sel_of (varrayptr0 r p) h
+let arrayptr_sel #a r = fun h -> sel_of (varrayptr0 r) h
+
+val intro_varrayptr
+  (#opened: _)
+  (#a: Type)
+  (r: t a)
+  (x: A.array a)
+  (p: perm)
+: SteelGhost unit opened
+    (ghost_vptr r.to `star` ghost_vptr r.rperm `star` A.varrayp x p)
+    (fun _ -> varrayptr r)
+    (fun h -> (
+      can_be_split (ghost_vptr r.to `star` ghost_vptr r.rperm `star` A.varrayp x p) (ghost_vptr r.to) /\
+      can_be_split (ghost_vptr r.to `star` ghost_vptr r.rperm `star` A.varrayp x p) (ghost_vptr r.rperm)
+    ) ==> (
+      let to = h (ghost_vptr r.to) in
+      x == array_of r to /\
+      p == h (ghost_vptr r.rperm)
+    ))
+    (fun h _ h' ->
+      let s' = h' (varrayptr r) in
+      s'.array == x /\
+      s'.perm == p /\
+      s'.contents == h (A.varrayp x p)
+    )
 
 let intro_varrayptr
+  #_ #a r x p
+=
+  reveal_star_3 (ghost_vptr r.to) (ghost_vptr r.rperm) (A.varrayp x p);
+  reveal_star (ghost_vptr r.to) (ghost_vptr r.rperm);
+  intro_vdep
+    (ghost_vptr r.to `star` ghost_vptr r.rperm)
+    (A.varrayp x p)
+    (varrayptr0_dep r);
+  intro_vrewrite
+    ((ghost_vptr r.to `star` ghost_vptr r.rperm) `vdep` varrayptr0_dep r)
+    (varrayptr0_rewrite r);
+  let g : Ghost.erased (v a) = gget (varrayptr0 r) in
+  assert (g.array == x);
+  assert (g.perm == p);
+  change_slprop_rel
+    (varrayptr0 r)
+    (varrayptr r)
+    (fun x y -> x == y)
+    (fun m -> ())
+
+[@@erasable]
+noeq
+type w (a: Type) = {
+  w_array: A.array a; 
+  w_perm: perm;
+}
+
+val elim_varrayptr
   (#opened: _)
   (#a: Type)
   (r: t a)
-  (p: perm)
-: SteelGhost unit opened
-    ((ghost_vptr r.to `vdep` varrayptr0_dep p r) `vrewrite` varrayptr0_rewrite p r)
-    (fun _ -> varrayptrp r p)
-    (fun _ -> True)
-    (fun h0 _ h1 -> h1 (varrayptrp r p) == h0 ((ghost_vptr r.to `vdep` varrayptr0_dep p r) `vrewrite` varrayptr0_rewrite p r))
-=
-  change_slprop_rel
-    ((ghost_vptr r.to `vdep` varrayptr0_dep p r) `vrewrite` varrayptr0_rewrite p r)
-    (varrayptrp r p)
-    (fun x y -> x == y)
-    (fun _ -> ())
+: SteelGhost (w a) opened
+    (varrayptr r)
+    (fun res -> ghost_vptr r.to `star` ghost_vptr r.rperm `star` A.varrayp res.w_array res.w_perm)
+    (fun h -> True)
+    (fun h res h' ->
+      let s = h (varrayptr r) in
+      can_be_split (ghost_vptr r.to `star` ghost_vptr r.rperm `star` A.varrayp res.w_array res.w_perm) (ghost_vptr r.to) /\
+      can_be_split (ghost_vptr r.to `star` ghost_vptr r.rperm `star` A.varrayp res.w_array res.w_perm) (ghost_vptr r.rperm) /\
+      res.w_array == s.array /\
+      res.w_array == array_of r (h' (ghost_vptr r.to)) /\
+      res.w_perm == h' (ghost_vptr r.rperm) /\
+      res.w_perm == s.perm /\
+      h' (A.varrayp res.w_array res.w_perm) == s.contents
+    )
 
 let elim_varrayptr
-  (#opened: _)
-  (#a: Type)
-  (r: t a)
-  (p: perm)
-: SteelGhost unit opened
-    (varrayptrp r p)
-    (fun _ -> (ghost_vptr r.to `vdep` varrayptr0_dep p r) `vrewrite` varrayptr0_rewrite p r)
-    (fun _ -> True)
-    (fun h0 _ h1 -> h0 (varrayptrp r p) == h1 ((ghost_vptr r.to `vdep` varrayptr0_dep p r) `vrewrite` varrayptr0_rewrite p r))
+  #_ #a r
 =
   change_slprop_rel
-    (varrayptrp r p)
-    ((ghost_vptr r.to `vdep` varrayptr0_dep p r) `vrewrite` varrayptr0_rewrite p r)
+    (varrayptr r)
+    (varrayptr0 r)
     (fun x y -> x == y)
-    (fun _ -> ())
-
-#push-options "--z3rlimit 32"
-let joinp #opened #a al ar p =
-  elim_varrayptr al p;
-  elim_vrewrite (ghost_vptr al.to `vdep` varrayptr0_dep p al) (varrayptr0_rewrite p al);
-  let g_al_to = elim_vdep (ghost_vptr al.to) (varrayptr0_dep p al) in
-  let al_to = ghost_read al.to in
-  let aal = array_of al al_to in
+    (fun m -> ());
+  elim_vrewrite
+    ((ghost_vptr r.to `star` ghost_vptr r.rperm) `vdep` varrayptr0_dep r)
+    (varrayptr0_rewrite r);
+  let to_perm = elim_vdep
+    (ghost_vptr r.to `star` ghost_vptr r.rperm)
+    (varrayptr0_dep r)
+  in
+  reveal_star (ghost_vptr r.to) (ghost_vptr r.rperm);
+  let to = ghost_read r.to in
+  let p = ghost_read r.rperm in
+  let res = {
+    w_array = array_of r to;
+    w_perm = p;
+  } in
   change_equal_slprop
-    (varrayptr0_dep p al (Ghost.reveal g_al_to))
-    (A.varrayp aal p);
-  elim_varrayptr ar p;
-  elim_vrewrite (ghost_vptr ar.to `vdep` varrayptr0_dep p ar) (varrayptr0_rewrite p ar);
-  let g_ar_to = elim_vdep (ghost_vptr ar.to) (varrayptr0_dep p ar) in
+    (varrayptr0_dep r to_perm)
+    (A.varrayp res.w_array res.w_perm);
+  reveal_star_3 (ghost_vptr r.to) (ghost_vptr r.rperm) (A.varrayp res.w_array res.w_perm);
+  res
+
+#push-options "--z3rlimit 16"
+let join #opened #a al ar =
+  let wl = elim_varrayptr al in
+  let p = ghost_read al.rperm in
+  change_equal_slprop
+    (A.varrayp wl.w_array wl.w_perm)
+    (A.varrayp wl.w_array p);
+  let wr = elim_varrayptr ar in
   let ar_to = ghost_read ar.to in
   ghost_free ar.to;
-  let aar = array_of ar ar_to in
+  ghost_free ar.rperm;
   change_equal_slprop
-    (varrayptr0_dep p ar (Ghost.reveal g_ar_to))
-    (A.varrayp aar p);
-  let aj = A.gjoin aal aar p in
+    (A.varrayp wr.w_array wr.w_perm)
+    (A.varrayp wr.w_array p);
+  let aj = A.gjoin wl.w_array wr.w_array p in
   let ar_to : U32.t = ar_to in
   let ar_to : to_t al.base al.from = ar_to in
   ghost_write al.to ar_to;
-  assert (Ghost.reveal aj == array_of al ar_to);
-  intro_vdep (ghost_vptr al.to) (A.varrayp aj p) (varrayptr0_dep p al);
-  intro_vrewrite (ghost_vptr al.to `vdep` varrayptr0_dep p al) (varrayptr0_rewrite p al);
-  intro_varrayptr al p
+  intro_varrayptr al aj p
 #pop-options
 
 let u32_bounded_add
@@ -165,42 +223,32 @@ let u32_bounded_add
 =
   x `U32.add` y
 
-#push-options "--z3rlimit 32"
+#push-options "--z3rlimit 16"
 #restart-solver
-let splitp #a x p i =
-  elim_varrayptr x p;
-  elim_vrewrite (ghost_vptr x.to `vdep` varrayptr0_dep p x) (varrayptr0_rewrite p x);
-  let x_to_1 : to_t x.base x.from = elim_vdep (ghost_vptr x.to) (varrayptr0_dep p x) in
-  let xa = array_of x x_to_1 in
+let split #a x i =
+  let w = elim_varrayptr x in
+  let p = w.w_perm in
   change_equal_slprop
-    (varrayptr0_dep p x (Ghost.reveal x_to_1))
-    (A.varrayp xa p);
-  let res2 : Ghost.erased (A.array a & A.array a) = A.gsplit0 p xa i in
+    (A.varrayp w.w_array w.w_perm)
+    (A.varrayp w.w_array p);
+  let res2 : Ghost.erased (A.array a & A.array a) = A.gsplit0 p w.w_array i in
   reveal_star (A.varrayp (A.pfst res2) p) (A.varrayp (A.psnd res2) p);
+  let x_to_1 = ghost_read x.to in
   let x_to_2 : Ghost.erased U32.t = Ghost.hide (Ghost.reveal x_to_1) in
   let j : to_v x.base x.from = u32_bounded_add x.from i x_to_2 in
   let x_to_3 : to_t x.base j = Ghost.hide (Ghost.reveal x_to_2) in
   ghost_write x.to j;
-  assert (A.pfst res2 == array_of x j);
-  intro_vdep
-    (ghost_vptr x.to)
-    (A.varrayp (A.pfst res2) p)
-    (varrayptr0_dep p x);
-  intro_vrewrite (ghost_vptr x.to `vdep` varrayptr0_dep p x) (varrayptr0_rewrite p x);
-  intro_varrayptr x p;
+  intro_varrayptr x (A.pfst res2) p;
   let to2 : ghost_ref (to_v x.base j) = ghost_alloc x_to_3 in
-  let res : t a = mk_t x.base j to2 in
-  let x_to_4 : to_t res.base res.from = Ghost.hide (Ghost.reveal x_to_3 <: U32.t) in
-  assert (A.psnd res2 == array_of res x_to_4);
+  let p2 : ghost_ref perm = ghost_alloc p in
+  let res : t a = mk_t x.base j to2 p2 in
   change_equal_slprop
     (ghost_vptr to2)
     (ghost_vptr res.to);
-  intro_vdep
-    (ghost_vptr res.to)
-    (A.varrayp (A.psnd res2) p)
-    (varrayptr0_dep p res);
-  intro_vrewrite (ghost_vptr res.to `vdep` varrayptr0_dep p res) (varrayptr0_rewrite p res);
-  intro_varrayptr res p;
+  change_equal_slprop
+    (ghost_vptr p2)
+    (ghost_vptr res.rperm);
+  intro_varrayptr res (A.psnd res2) p;
   return res
 #pop-options
 
@@ -211,68 +259,54 @@ let alloc
   let ar = A.alloc2 x n in
   let n2 : to_t ar.A.base 0ul = n in
   let to : ghost_ref (to_v ar.A.base 0ul) = ghost_alloc n2 in
+  let perm : ghost_ref perm = ghost_alloc full_perm in
   let res = {
     base = ar.A.base;
     from = 0ul;
     to = to;
+    rperm = perm;
   } in
-  assert (array_of res n2 == ar);
   change_equal_slprop
     (ghost_vptr to)
     (ghost_vptr res.to);
-  intro_vdep
-    (ghost_vptr res.to)
-    (A.varray ar)
-    (varrayptr0_dep _ res);
-  intro_vrewrite (ghost_vptr res.to `vdep` varrayptr0_dep _ res) (varrayptr0_rewrite _ res);
-  intro_varrayptr res _;
+  change_equal_slprop
+    (ghost_vptr perm)
+    (ghost_vptr res.rperm);
+  intro_varrayptr res ar full_perm;
   return res
 
-let indexp
-  #a r p i
+let index
+  #a r i
 =
-  elim_varrayptr r p;
-  elim_vrewrite (ghost_vptr r.to `vdep` varrayptr0_dep p r) (varrayptr0_rewrite p r);
-  let g = elim_vdep (ghost_vptr r.to) (varrayptr0_dep p r) in
+  let w = elim_varrayptr r in
   let to = ghost_read r.to in
   let ar = array_of r to in
   change_equal_slprop
-    (varrayptr0_dep p r (Ghost.reveal g))
-    (A.varrayp ar p);
-  let res = A.indexp ar p i in
-  intro_vdep
-    (ghost_vptr r.to)
-    (A.varrayp ar p)
-    (varrayptr0_dep p r);
-  intro_vrewrite (ghost_vptr r.to `vdep` varrayptr0_dep p r) (varrayptr0_rewrite p r);
-  intro_varrayptr r p;
+    (A.varrayp w.w_array w.w_perm)
+    (A.varrayp ar w.w_perm);
+  let res = A.indexp ar w.w_perm i in
+  intro_varrayptr r ar w.w_perm;
   return res
 
 let upd
   #a r i x
 =
-  elim_varrayptr r _;
-  elim_vrewrite (ghost_vptr r.to `vdep` varrayptr0_dep _ r) (varrayptr0_rewrite _ r);
-  let to = elim_vdep (ghost_vptr r.to) (varrayptr0_dep _ r) in
+  let w = elim_varrayptr r in
+  let to = ghost_read r.to in
   let ar = array_of r to in
   change_equal_slprop
-    (varrayptr0_dep _ r (Ghost.reveal to))
-    (A.varray ar);
+    (A.varrayp w.w_array w.w_perm)
+    (A.varrayp ar full_perm);
   A.upd ar i x;
-  intro_vdep
-    (ghost_vptr r.to)
-    (A.varray ar)
-    (varrayptr0_dep _ r);
-  intro_vrewrite (ghost_vptr r.to `vdep` varrayptr0_dep _ r) (varrayptr0_rewrite _ r);
-  intro_varrayptr r _
+  intro_varrayptr r ar full_perm
 
 let free #a r =
-  elim_varrayptr r _;
-  elim_vrewrite (ghost_vptr r.to `vdep` varrayptr0_dep _ r) (varrayptr0_rewrite _ r);
-  let to = elim_vdep (ghost_vptr r.to) (varrayptr0_dep _ r) in
+  let w = elim_varrayptr r in
+  ghost_free r.rperm;
+  let to = ghost_read r.to in
   ghost_free r.to;
   let ar = array_of r to in
   change_equal_slprop
-    (varrayptr0_dep _ r to)
+    (A.varrayp w.w_array w.w_perm)
     (A.varray ar);
   A.free ar
