ulib/experimental/Steel.ArrayPtr.fsti
@@ -42,22 +42,20 @@ val t (t:Type u#0) : Type u#0
 noeq type v (t: Type u#0) = {
   array: A.array t;                      (* spatial permission range *)
   contents: Seq.lseq t (A.length array); (* actual contents *)
+  perm: perm;                            (* temporal permission *)
 }
 
-val is_arrayptr (#a:Type0) (r:t a) (p: perm) : slprop u#1
-val arrayptr_sel (#a:Type0) (r:t a) (p: perm) : selector (v a) (is_arrayptr r p)
+val is_arrayptr (#a:Type0) (r:t a) : slprop u#1
+val arrayptr_sel (#a:Type0) (r:t a) : selector (v a) (is_arrayptr r)
 
 [@@ __steel_reduce__]
-let varrayptr' #a r p : vprop' =
-  {hp = is_arrayptr r p;
+let varrayptr' #a r : vprop' =
+  {hp = is_arrayptr r;
    t = v a;
-   sel = arrayptr_sel r p}
+   sel = arrayptr_sel r}
 
 [@@ __steel_reduce__]
-let varrayptrp r p = VUnit (varrayptr' r p)
-
-[@@ __steel_reduce__]
-let varrayptr r = varrayptrp r full_perm
+let varrayptr r = VUnit (varrayptr' r)
 
 [@@ __steel_reduce__]
 let sel (#a:Type) (#p:vprop) (r:t a)
@@ -68,51 +66,24 @@ let sel (#a:Type) (#p:vprop) (r:t a)
 
 (* Splitting an array (inspired from Steel.Array) *)
 
-val joinp (#opened: _) (#a:Type) (al ar:t a) (p: perm)
-  : SteelGhost unit opened
-          (varrayptrp al p `star` varrayptrp ar p)
-          (fun _ -> varrayptrp al p)
-          (fun h -> A.adjacent (h (varrayptrp al p)).array (h (varrayptrp ar p)).array)
-          (fun h _ h' ->
-            let cl = h (varrayptrp al p) in
-            let cr = h (varrayptrp ar p) in
-            let c' = h' (varrayptrp al p) in
-            A.merge_into cl.array cr.array c'.array /\
-            c'.contents == cl.contents `Seq.append` cr.contents
-          )
-
-let join (#opened: _) (#a:Type) (al ar:t a)
+val join (#opened: _) (#a:Type) (al ar:t a)
   : SteelGhost unit opened
           (varrayptr al `star` varrayptr ar)
           (fun _ -> varrayptr al)
-          (fun h -> A.adjacent (h (varrayptr al)).array (h (varrayptr ar)).array)
+          (fun h ->
+            A.adjacent (h (varrayptr al)).array (h (varrayptr ar)).array /\
+            (h (varrayptr al)).perm == (h (varrayptr ar)).perm
+          )
           (fun h _ h' ->
             let cl = h (varrayptr al) in
             let cr = h (varrayptr ar) in
             let c' = h' (varrayptr al) in
             A.merge_into cl.array cr.array c'.array /\
+            c'.perm == cl.perm /\
             c'.contents == cl.contents `Seq.append` cr.contents
           )
-=
-  joinp _ _ _
 
-val splitp (#a:Type) (x: t a) (p: perm) (i:U32.t)
-  : Steel (t a)
-          (varrayptrp x p)
-          (fun res -> varrayptrp x p `star` varrayptrp res p)
-          (fun h -> U32.v i <= A.length (h (varrayptrp x p)).array)
-          (fun h res h' ->
-            let s = h (varrayptrp x p) in
-            let sl = h' (varrayptrp x p) in
-            let sr = h' (varrayptrp res p) in
-            U32.v i <= A.length s.array /\
-            A.merge_into sl.array sr.array s.array /\
-            sl.contents == Seq.slice s.contents 0 (U32.v i) /\
-            sr.contents == Seq.slice s.contents (U32.v i) (A.length s.array) /\
-            s.contents == sl.contents `Seq.append` sr.contents
-          )
-
-let split (#a:Type) (x: t a) (i:U32.t)
+val split (#a:Type) (x: t a) (i:U32.t)
   : Steel (t a)
           (varrayptr x)
           (fun res -> varrayptr x `star` varrayptr res)
@@ -123,12 +94,12 @@ let split (#a:Type) (x: t a) (i:U32.t)
             let sr = h' (varrayptr res) in
             U32.v i <= A.length s.array /\
             A.merge_into sl.array sr.array s.array /\
+            sl.perm == s.perm /\
+            sr.perm == s.perm /\
             sl.contents == Seq.slice s.contents 0 (U32.v i) /\
             sr.contents == Seq.slice s.contents (U32.v i) (A.length s.array) /\
             s.contents == sl.contents `Seq.append` sr.contents
           )
-=
-  splitp _ _ i
 
 val alloc (#a:Type) (x:a) (n:U32.t)
   : Steel (t a)
@@ -137,21 +108,11 @@ val alloc (#a:Type) (x:a) (n:U32.t)
              (requires fun _ -> True)
              (ensures fun _ r h1 ->
                (h1 (varrayptr r)).contents == Seq.create (U32.v n) x /\
+               (h1 (varrayptr r)).perm == full_perm /\
                A.freeable (h1 (varrayptr r)).array
              )
 
-val indexp (#a:Type) (r: t a) (p: perm) (i:U32.t)
-  : Steel a
-             (varrayptrp r p)
-             (fun _ -> varrayptrp r p)
-             (requires fun h -> U32.v i < A.length (h (varrayptrp r p)).array)
-             (ensures fun h0 y h1 ->
-               let s = h0 (varrayptrp r p) in
-               h1 (varrayptrp r p) == s /\
-               U32.v i < A.length s.array /\
-               y == Seq.index s.contents (U32.v i))
-
-let index (#a:Type) (r: t a) (i:U32.t)
+val index (#a:Type) (r: t a) (i:U32.t)
   : Steel a
              (varrayptr r)
              (fun _ -> varrayptr r)
@@ -161,18 +122,20 @@ let index (#a:Type) (r: t a) (i:U32.t)
                h1 (varrayptr r) == s /\
                U32.v i < A.length s.array /\
                y == Seq.index s.contents (U32.v i))
-=
-  indexp _ _ i
 
 val upd (#a:Type) (r: t a) (i:U32.t) (x:a)
   : Steel unit
              (varrayptr r)
              (fun _ -> varrayptr r)
-             (requires fun h -> U32.v i < A.length (h (varrayptr r)).array)
+             (requires fun h ->
+               (h (varrayptr r)).perm == full_perm /\
+               U32.v i < A.length (h (varrayptr r)).array
+             )
              (ensures fun h0 _ h1 ->
                let s = h0 (varrayptr r) in
                let s' = h1 (varrayptr r) in
                s'.array == s.array /\
+               s'.perm == full_perm /\
                U32.v i < A.length s.array /\
                s'.contents == Seq.upd s.contents (U32.v i) x)
 
@@ -180,5 +143,8 @@ val free (#a:Type) (r:t a)
   : Steel unit
              (varrayptr r)
              (fun _ -> emp)
-             (requires fun h -> A.freeable (h (varrayptr r)).array)
+             (requires fun h ->
+               (h (varrayptr r)).perm == full_perm /\
+               A.freeable (h (varrayptr r)).array
+             )
              (ensures fun _ _ _ -> True)
